Examples working with arraystructs

ulib/experimental/Steel.PCM.ArrayStruct.fst
@@ -20,6 +20,7 @@ module DepMap = FStar.DependentMap
 
 open FStar.FunctionalExtensionality
 open Steel.PCM
+open Steel.PCM.Unitless
 
 type usize = U32.t
 let v_usize = U32.v
@@ -79,74 +80,10 @@ unfold let struct_field_type
   : Tot (Type u#a) =
   struct_field_type' field_descriptors array_struct_type field
 
-/// The descriptor does not contain any information on the PCM that will govern the arraystruct
-/// values. Here, we are confronted to several choices :
-///   * We could discharge to the user the burden of defining completely the pcm corresponding to
-///   a particular, often recursive, descriptor. This is the most expressive option but defining and
-///   proving the laws of such a PCM is very tedious, and we want to help the user to define their
-///   PCM for their arraystruct.
-///   * The second option is to define a "pointwise" PCM for every arraystruct, by just taking for its
-///   laws and operations the combination of all the laws and operations of all the PCMs stored
-///   at the leaves (DBase case) of the arraystruct. This options seems sensible but this "pointwise"
-///   PCM is actually not very useful: such a PCM does not let the user define memory partition schemes
-///   like "thread A posesses the first two fields of the struct, and thread B posesses the rest".
-///   * The third option is in the middle: letting the user define their own PCM, but with some
-///   help from the arraystruct library such that common patterns are handled easily.
-///
-/// The rest of the library chooses the third option. We assume that common pattern for defining PCM on
-/// arraystructs is to define partition of structs and arrays that depend mostly on the indexes of
-/// the arrays and the fields of the struct rather than the actual values stored inside the cells of
-/// the arrays or the fields of the struct. For instance, splitting an array into two contiguous
-/// halves, or splitting the fields of a struct.
-/// To define such "value-agnostic" PCMs, we will require the user to define their own PCM based purely
-/// on restricted information:
-///   * the opaque type of the array cell values and struct fields (parametricity forbids
-///   value-dependent conditions);
-///   * the length of the array or the name of the fields of the struct;
-///   * to ensure recursivity, the array-struct for the "level below" of the arraystruct structure.
-///
-/// This may help to understand the definition below.
-noeq type array_struct_nested_pcm : Type u#(a+1) =
-  | PBase:
-    a: Type u#a ->
-    pcm: pcm a ->
-    array_struct_nested_pcm
-  | PArray:
-    cell_type: Type u#a ->
-    len: usize ->
-    cell_nested_pcm: array_struct_nested_pcm u#a ->
-    array_pcm: (pcm cell_type -> pcm (array_type cell_type len)) ->
-    array_struct_nested_pcm
-  | PStruct:
-    field_types: (field_id ^-> Type u#a) ->
-    field_nested_pcms: (field:field_id -> array_struct_nested_pcm u#a) ->
-    struct_pcm: ((field:field_id -> pcm (field_types field)) -> pcm (struct_type field_types)) ->
-    array_struct_nested_pcm
-
-/// Because F* does not support induction-recursion, we had to resort to defining another inductive
-/// type for the nested pcm and thus have to define this recusrive "sync" predicate that ensures that
-/// the nested PCM and the descriptor match.
-let rec nested_pcm_sync
-  (descriptor: array_struct_descriptor)
-  (nested_pcm: array_struct_nested_pcm) : GTot prop (decreases descriptor) =
-  match descriptor, nested_pcm with
-  | DBase da, PBase va _ ->
-    da == va
-  | DArray cell_descriptor dlen, PArray cell_type plen cell_nested_pcm _  ->
-    dlen = plen /\ cell_type == array_struct_type cell_descriptor /\
-    cell_descriptor `nested_pcm_sync` cell_nested_pcm
-  | DStruct field_descriptors, PStruct field_types field_nested_pcms struct_pcm ->
-    field_types == struct_field_type field_descriptors /\
-    (forall (field: field_id). begin
-      FStar.WellFounded.axiom1 field_descriptors field;
-      field_descriptors field `nested_pcm_sync` field_nested_pcms field
-    end)
-  | _ -> False
-
 noeq type array_struct : Type u#(a+1) =
   | ArrayStruct:
     descriptor: array_struct_descriptor u#a ->
-    nested_pcm: array_struct_nested_pcm u#a{descriptor `nested_pcm_sync` nested_pcm} ->
+    pcm: unitless_pcm (array_struct_type descriptor) ->
     value: array_struct_type descriptor ->
     array_struct
 
@@ -165,106 +102,50 @@ let struct_field_type_unroll_lemma
     compute ()
   end
 
-/// From the PCM builders stored inside the nested PCM, we can derive a PCM for the whole value stored
-/// inside the arraystruct.
-let rec nested_pcm_to_pcm
-  (descriptor: array_struct_descriptor u#a)
-  (nested_pcm: array_struct_nested_pcm u#a{descriptor `nested_pcm_sync` nested_pcm})
-    : Tot (pcm (array_struct_type descriptor)) (decreases descriptor) =
-  match descriptor, nested_pcm with
-  | _, PBase _ pcm -> pcm
-  | DArray cell_descriptor _, PArray cell_type _ cell_nested_pcm array_pcm ->
-    array_pcm (nested_pcm_to_pcm cell_descriptor cell_nested_pcm)
-  | DStruct field_descriptors, PStruct field_types field_nested_pcms struct_pcm ->
-    assert(descriptor `nested_pcm_sync` nested_pcm);
-    assume(field_types == struct_field_type field_descriptors); // Why can't F* find this???
-    struct_field_type_unroll_lemma field_descriptors;
-    struct_pcm (fun field ->
-      FStar.WellFounded.axiom1 field_descriptors field;
-      nested_pcm_to_pcm (field_descriptors field) (field_nested_pcms field)
-    )
-
 /// Composability is then based on the composability of the nested PCM.
 let composable_array_struct : symrel u#(a+1) (array_struct u#a) = fun (s0 s1: array_struct u#a) ->
-  s0.descriptor == s1.descriptor /\ s0.nested_pcm == s1.nested_pcm /\
-  composable (nested_pcm_to_pcm s0.descriptor s0.nested_pcm) s0.value s1.value
+  s0.descriptor == s1.descriptor /\ s0.pcm == s1.pcm /\
+  s0.pcm.unitless_p.unitless_composable s0.value s1.value
 
 let compose_array_struct
   (s0: array_struct u#a)
   (s1: array_struct u#a{s0 `composable_array_struct` s1})
     : array_struct u#a
   =
-  let new_val = op (nested_pcm_to_pcm s0.descriptor s0.nested_pcm) s0.value s1.value in
-  ArrayStruct s0.descriptor s0.nested_pcm new_val
-
-let unit_pcm' : pcm' u#a (Univ.raise_t u#0 u#a unit) = {
-    composable = (fun _ _ -> True);
-    op = (fun _ _ -> Univ.raise_val u#0 u#a () );
-    one =  Univ.raise_val u#0 u#a ()
-  }
-
-let higher_unit (x: Univ.raise_t u#0 u#a unit) : Lemma (x == Univ.raise_val u#0 u#a ()) =
-  let aux (_ : squash (x =!= Univ.raise_val u#0 u#a ())) : Lemma (False) =
-      let x0 = Univ.downgrade_val u#0 u#a x in
-      assert(x0 == ())
-  in
-  Classical.excluded_middle (x == Univ.raise_val u#0 u#a ());
-  Classical.or_elim
-    #(x == Univ.raise_val u#0 u#a ())
-    #(x =!= Univ.raise_val u#0 u#a ())
-    #(fun _ -> unit_pcm'.composable x unit_pcm'.one /\ unit_pcm'.op x unit_pcm'.one == x)
-    (fun _ -> ())
-    (fun _ -> aux ())
-
-let unit_pcm : pcm u#a (Univ.raise_t u#0 u#a unit)  = {
-  p = unit_pcm' u#a;
-  comm = (fun _ _  -> ());
-  assoc = (fun _ _ _ -> ());
-  assoc_r = (fun _ _ _ -> ());
-  is_unit = (fun x -> higher_unit x)
-}
-
-let array_struct_unit : array_struct u#a =
-  ArrayStruct
-    (DBase (Univ.raise_t u#0 u#a unit))
-    (PBase (Univ.raise_t u#0 u#a unit) unit_pcm)
-    (Univ.raise_val u#0 u#a ())
+  let new_val = s0.pcm.unitless_p.unitless_op s0.value s1.value in
+  ArrayStruct s0.descriptor s0.pcm new_val
 
 #set-options "--print_universes --print_implicits"
 
-let array_struct_pcm' : pcm' u#(a+1) (array_struct u#a) = {
-  composable = composable_array_struct u#a;
-  op = compose_array_struct u#a;
-  one = array_struct_unit u#a;
+let array_struct_unitless_pcm' : unitless_pcm' u#(a+1) (array_struct u#a) = {
+  unitless_composable = composable_array_struct u#a;
+  unitless_op = compose_array_struct u#a;
 }
 
-let array_struct_pcm : pcm u#(a+1) (array_struct u#a) = {
-  p = array_struct_pcm' u#a;
-  comm = (fun _ _  -> admit());
-  assoc = (fun _ _ _ -> admit());
-  assoc_r = (fun _ _ _ -> admit());
-  is_unit = (fun x -> admit());
+let array_struct_unitless_pcm : unitless_pcm u#(a+1) (array_struct u#a) = {
+  unitless_p = array_struct_unitless_pcm' u#a;
+  unitless_comm = (fun s0 s1  -> s0.pcm.unitless_comm s0.value s1.value);
+  unitless_assoc = (fun s0 s1 s2 -> s0.pcm.unitless_assoc s0.value s1.value s2.value);
+  unitless_assoc_r = (fun s0 s1 s2 -> s0.pcm.unitless_assoc_r s0.value s1.value s2.value);
 }
 
-////////////////////////////////////////////////////////////////////
-// Examples
-////////////////////////////////////////////////////////////////////
+let array_struct_pcm : pcm u#(a+1) (option u#(a+1) (array_struct u#a)) =
+  to_full_pcm_with_unit array_struct_unitless_pcm
 
-open Steel.PCM.FractionalPermission
-open Steel.PCM.Base
-
-#set-options "--print_implicits --print_universes"
+////////////////////////////////////////////////////////////////////
+// PCM builders
+////////////////////////////////////////////////////////////////////
 
 let pointwise_array_pcm
   (cell_type: Type u#a)
   (len: usize)
-  (base_pcm: pcm cell_type)
-    : pcm (array_type cell_type len)
+  (base_pcm: unitless_pcm cell_type)
+    : unitless_pcm (array_type cell_type len)
   =
   let composable_cell (x y: array_type cell_type len) (i:nat{i < v_usize len}) : prop =
     let xi = Seq.index x i in
     let yi = Seq.index y i in
-    composable base_pcm xi yi
+    base_pcm.unitless_p.unitless_composable xi yi
   in
   let composable : symrel (array_type cell_type len) =
     fun x y -> forall (i:nat{i < v_usize len}). composable_cell x y i
@@ -277,117 +158,122 @@ let pointwise_array_pcm
     Seq.init (v_usize len) (fun i ->
       let xi = Seq.index x i in
       let yi = Seq.index y i in
-      op base_pcm xi yi
+      base_pcm.unitless_p.unitless_op xi yi
     )
   in
-  let unit : array_type cell_type len =
-    Seq.init (v_usize len) (fun _ -> base_pcm.p.one)
-  in
-  let pcm' : pcm' (array_type cell_type len) = {
-    composable;
-    op = compose;
-    one = unit;
+  let pcm' : unitless_pcm' (array_type cell_type len) = {
+    unitless_composable = composable;
+    unitless_op = compose;
   } in
   {
-    p = pcm';
-    comm = (fun _ _ -> admit());
-    assoc = (fun _ _ _ -> admit());
-    assoc_r = (fun _ _ _ -> admit());
-    is_unit = (fun _ -> admit())
+    unitless_p = pcm';
+    (* The proofs here should simply follow by generalization for all indexes *)
+    unitless_comm = (fun x y -> admit());
+    unitless_assoc = (fun _ _ _ -> admit());
+    unitless_assoc_r = (fun _ _ _ -> admit());
   }
 
-#push-options "--fuel 2"
+let pointwise_struct_pcm
+  (field_types: field_id -> Type u#a)
+  (base_pcms: (field:field_id -> unitless_pcm (field_types field)))
+    : unitless_pcm (struct_type field_types)
+  =
+  let composable_field (field: field_id) (x y: struct_type field_types) : prop =
+    let xf = DepMap.sel x field in
+    let yf = DepMap.sel y field in
+    (base_pcms field).unitless_p.unitless_composable xf yf
+  in
+  let composable : symrel (struct_type field_types) =
+    fun x y -> forall (field: field_id). composable_field field x y
+  in
+  let compose
+    (x: struct_type field_types)
+    (y: struct_type field_types{composable x y})
+      : struct_type field_types
+    =
+    DepMap.create (fun field ->
+      let xf = DepMap.sel x field in
+      let yf = DepMap.sel y field in
+      (base_pcms field).unitless_p.unitless_op xf yf
+    )
+  in
+  let pcm' : unitless_pcm' (struct_type field_types) = {
+    unitless_composable = composable;
+    unitless_op = compose;
+  } in
+  {
+    unitless_p = pcm';
+    (* The proofs here should simply follow by generalization for all fields *)
+    unitless_comm = (fun x y -> admit());
+    unitless_assoc = (fun _ _ _ -> admit());
+    unitless_assoc_r = (fun _ _ _ -> admit());
+  }
+
+////////////////////////////////////////////////////////////////////
+// Examples
+////////////////////////////////////////////////////////////////////
+
+open Steel.PCM.FractionalPermission
+open Steel.PCM.Unitless.Base
+
 let array_with_frac_perm_on_all_indexes (t: Type u#a) (len: usize) (v: t) : array_struct u#a
   =
   ArrayStruct
     (DArray (DBase (with_perm u#a t)) len)
-    (PArray (with_perm u#a t) len
-      (PBase (with_perm u#a t) (frac_perm_pcm u#a v))
-      (pointwise_array_pcm (with_perm u#a t) len)
-    )
+    (pointwise_array_pcm (with_perm t) len frac_perm_pcm)
     (Seq.init u#a (v_usize len) (fun _ -> { value = v; perm = perm_one} ))
-#pop-options
 
-#push-options "--fuel 2"
 let immutable_splittable_array (t: Type u#a) (len: usize) (v: t) : array_struct u#a
   =
   ArrayStruct
-    (DArray (DBase (option t)) len)
-    (PArray (option t) len
-       (PBase (option t) immutable_pcm)
-       (pointwise_array_pcm (option t) len)
-    )
-    (Seq.init u#a (v_usize len) (fun _ -> Some v))
-#pop-options
+    (DArray (DBase t) len)
+    (pointwise_array_pcm t len immutable_unitless_pcm)
+    (Seq.init u#a (v_usize len) (fun _ -> v))
 
-let pointwise_array_pcm_with_prefix_pcm
-  (cell_type: Type u#a)
-  (len: usize)
-  (prefix_len:nat{prefix_len < v_usize len})
-  (prefix_pcm: pcm cell_type)
-  (base_pcm: pcm cell_type)
-    : pcm (array_type cell_type len)
-  =
-  let composable_cell (x y: array_type cell_type len) (i:nat{i < v_usize len}) : prop =
-    let xi = Seq.index x i in
-    let yi = Seq.index y i in
-    if i < prefix_len then
-      composable prefix_pcm xi yi
+let two_fields_restricted_func
+  (#a: Type u#a)
+  (field1: string)
+  (field2: string{field2 <> field1})
+  (value1 value2 by_default: a)
+  : (field_id ^-> a) =
+  on _ (fun field ->
+    if field = field1 then value1
+    else if field = field2 then value2
+    else by_default
+  )
+
+#push-options "--fuel 2 --ifuel 2"
+let two_fields_dep_map
+  (a: field_id -> Type u#a)
+  (field1: string)
+  (field2: string{field2 <> field1})
+  (value1: a field1)
+  (value2: a field2)
+  (by_default: (field:field_id{field <> field1 /\ field <> field2} -> a field))
+  : (DepMap.t field_id a) =
+  DepMap.create #field_id #a (fun field ->
+    if field = field1 then begin admit(); value1 end (* Why can't F* find this ? *)
+    else if field = field2 then begin admit(); value2 end
+    else by_default field
+  )
+
+
+let point_2d : array_struct =
+  let field_descriptors =
+    two_fields_restricted_func "x" "y" (DBase int) (DBase int) (DBase unit)
+  in
+  let field_types : (field_id -> Type0) = struct_field_type field_descriptors in
+  let field_pcms : (field:field_id -> unitless_pcm (field_types field)) =
+    fun field ->
+    if field = "x" then
+      exclusive_unitless_pcm
+    else if field = "y" then
+      immutable_unitless_pcm
     else
-      composable base_pcm xi yi
+      exclusive_unitless_pcm
   in
-  let composable_array : symrel (array_type cell_type len) =
-    fun x y -> forall (i:nat{i < v_usize len}). composable_cell x y i
-  in
-  let compose
-    (x: array_type cell_type len)
-    (y: array_type cell_type len{composable_array x y})
-      : array_type cell_type len
-    =
-    Seq.init (v_usize len) (fun i ->
-      let xi = Seq.index x i in
-      let yi = Seq.index y i in
-      if i < prefix_len then begin
-        assume(composable prefix_pcm xi yi);
-        op prefix_pcm xi yi
-      end else
-        op base_pcm xi yi
-    )
-  in
-  let unit : array_type cell_type len =
-    Seq.init (v_usize len) (fun i ->
-       if i < prefix_len then
-         prefix_pcm.p.one
-       else
-        base_pcm.p.one
-    )
-  in
-  let pcm' : pcm' (array_type cell_type len) = {
-    composable = composable_array;
-    op = compose;
-    one = unit;
-  } in
-  {
-    p = pcm';
-    comm = (fun _ _ -> admit());
-    assoc = (fun _ _ _ -> admit());
-    assoc_r = (fun _ _ _ -> admit());
-    is_unit = (fun _ -> admit())
-  }
-
-#push-options "--fuel 2"
-let array_with_frac_perms_and_freezable_prefix
-  (t: Type u#a)
-  (len: usize)
-  (prefix_len: usize)
-  (v: t)
-    : array_struct u#a
-  =
+  struct_field_type_unroll_lemma field_descriptors;
   ArrayStruct
-    (DArray (DBase (with_perm u#a t)) len)
-    (PArray (with_perm u#a t) len
-      (PBase (with_perm u#a t) (frac_perm_pcm u#a v))
-      (pointwise_array_pcm_wi (with_perm u#a t) len)
-    )
-    (Seq.init u#a (v_usize len) (fun _ -> { value = v; perm = perm_one} ))
-#pop-options
+    (DStruct field_descriptors)
+    (pointwise_struct_pcm field_types field_pcms)
+    (two_fields_dep_map field_types "x" "y" 0 1 (fun _ -> ()))
